examples/max/max.dfy
@@ -44,6 +44,16 @@ lemma post_max_point_3(a:int, b:int, m:int)
     ensures !post_max(a, b, m)
 {}
 
+lemma post_max_vertical_1(a:int, b:int, m:int)
+    requires m != a && m != b
+    ensures !post_max(a, b, m)
+{}
+
+lemma post_max_vertical_1'(a:int, b:int, m:int)
+    requires post_max(a, b, m)
+    ensures m == a || m == b
+{}
+
 // to check if it is implementable
 lemma post_max_realistic_1(a:int, b:int, m:int)
     requires a > b
@@ -76,3 +86,23 @@ lemma max_deterministic'(a:int, b:int, m:int, m':int)
     requires m != m'
     ensures !post_max(a, b, m) || !post_max(a, b, m')
 {}
+
+
+
+lemma lemmaInvTheProposerOfAnyValidBlockInAnHonestBlockchailnIsInTheSetOfValidatorsHelper6Helper<T>(
+        s: seq<int>,
+        b: int,
+        i: nat
+    )
+    requires |s| > i 
+    requires b == s[i]
+    ensures s[..i] + [b] == s[..i+1]
+    {  }
+
+lemma multisetEquality(m1:multiset<int>, m2:multiset<int>, m3:multiset<int>, m4:multiset<int>)
+   requires m1 > m2 + m3
+   requires m1 == m2 + m4
+   ensures m3 < m4
+{
+    assert m3 < m1 - m2;
+}
